Merge _dev into _dev_frodo and revise Lib.Buffer

lib/fst/Lib.Buffer.fst
@@ -1,7 +1,5 @@
 module Lib.Buffer
 
-open FStar.HyperStack
-open FStar.HyperStack.ST
 open FStar.Mul
 
 open Lib.IntTypes
@@ -20,99 +18,95 @@ module ByteSeq = Lib.ByteSequence
 
 #reset-options "--z3rlimit 100 --max_fuel 0 --max_ifuel 0"
 
-let length #a b = B.length b
+let modifies_preserves_live #t #a b l h0 h1 = ()
+let modifies_includes l1 l2 h0 h1 = ()
+let modifies_trans l1 l2 h0 h1 h2 = ()
+let live_sub #t #a #len b start n h = ()
+let modifies_sub #t #a #len b start n h0 h1 = ()
 
-let ilength #a b = IB.length b
+let as_seq_gsub #t #a #len h b start n = ()
 
-let as_seq_gsub #a #len h b start n = ()
+let sub #t #a #len b start n =
+  match t with
+  | MUT -> B.sub (b <: buffer a) start n
+  | IMMUT -> IB.isub (b <: ibuffer a) start n
 
-let sub #a #len #olen b start n =
-  B.sub b (size_to_UInt32 start) (size_to_UInt32 n)
-
-let as_seq_igsub #a #len h b start n = ()
-
-let isub #a #len #olen b start n =
-  IB.isub b (size_to_UInt32 start) (size_to_UInt32 n)
-
-let index #a #len b i =
-  B.index b (size_to_UInt32 i)
-
-let iindex #a #len b i =
-  IB.index b (size_to_UInt32 i)
+let index #t #a #len b i =
+  match t with
+  | MUT -> B.index (b <: buffer a) i
+  | IMMUT -> IB.index (b <: ibuffer a) i
 
 let upd #a #len b i v =
-  B.upd b (size_to_UInt32 i) v
+  let h0 = ST.get() in
+  B.upd (b <: buffer a) i v;
+  let h1 = ST.get() in
+  assert (B.modifies (loc b) h0 h1);
+  assert (modifies (loc b) h0 h1)
 
-let bget #a #len h b i =
-  FStar.Seq.index #a (B.as_seq h b) i
+let bget_as_seq #t #a #len h b i = ()
 
-let ibget #a #len h b i =
-  FStar.Seq.index #a (IB.as_seq h b) i
-
-let create #a #len clen init =
-  B.alloca init (normalize_term (size_to_UInt32 clen))
+let create #a clen init =
+  B.alloca init (normalize_term clen)
 
 let createL #a init =
   B.alloca_of_list init
 
-let recall #a #len b = B.recall b
-
 #set-options "--max_fuel 1"
 
 let createL_global #a init =
-  B.gcmalloc_of_list HyperStack.root init
-
-let icreateL_global #a init =
   IB.igcmalloc_of_list #a root init
 
 let recall_contents #a #len b s =
-  B.recall_p b (cpred s)
+  B.recall_p (b <: ibuffer a) (cpred s)
 
-let copy #a #len o clen i =
-  let h0 = ST.get () in
-  LowStar.BufferOps.blit i (size_to_UInt32 (size 0)) o (size_to_UInt32 (size 0)) (size_to_UInt32 clen);
-  let h1 = ST.get () in
-  assert (Seq.slice #a #len (B.as_seq h1 o) 0 len == Seq.slice #a #len (B.as_seq h0 i) 0 len)
-
-let icopy #a #len o clen i =
-  let h0 = ST.get () in
-  LowStar.BufferOps.blit i (size_to_UInt32 (size 0)) o (size_to_UInt32 (size 0)) (size_to_UInt32 clen);
-  let h1 = ST.get () in
-  assert (Seq.slice #a #len (B.as_seq h1 o) 0 len == Seq.slice #a #len (B.as_seq h0 i) 0 len)
+let copy #t #a #len o i =
+  match t with
+  | MUT ->
+    let h0 = ST.get () in
+    LowStar.BufferOps.blit (i <: buffer a) 0ul (o <: buffer a) 0ul len;
+    let h1 = ST.get () in
+    assert (Seq.slice (as_seq h1 o) 0 (v len) == Seq.slice (as_seq h0 i) 0 (v len))
+  | IMMUT ->
+    let h0 = ST.get () in
+    LowStar.BufferOps.blit (i <: ibuffer a) 0ul (o <: buffer a) 0ul len;
+    let h1 = ST.get () in
+    assert (Seq.slice (as_seq h1 o) 0 (v len) == Seq.slice (as_seq h0 i) 0 (v len))
 
 let memset #a #blen b init len =
-  B.fill #a b init len
+  B.fill #a (b <: buffer a) init len
 
 #set-options "--max_fuel 0"
 
-let update_sub #a #len dst start n src =
+let update_sub #t #a #len dst start n src =
+  match t with
+  | MUT ->
   let h0 = ST.get () in
-  LowStar.BufferOps.blit src 0ul dst (size_to_UInt32 start) (size_to_UInt32 n);
+  LowStar.BufferOps.blit (src <: buffer a) 0ul (dst <: buffer a) (size_to_UInt32 start) (size_to_UInt32 n);
   let h1 = ST.get () in
   assert (forall (k:nat{k < v n}). bget h1 dst (v start + k) == bget h0 src k);
   FStar.Seq.lemma_eq_intro
-    (B.as_seq h1 dst)
-    (Seq.update_sub #a #len (B.as_seq h0 dst) (v start) (v n) (B.as_seq h0 src))
-
-let update_isub #a #len dst start n src =
+    (as_seq h1 dst)
+    (Seq.update_sub #a #(v len) (as_seq h0 dst) (v start) (v n) (as_seq h0 src))
+  | IMMUT ->
   let h0 = ST.get () in
-  LowStar.BufferOps.blit src 0ul dst (size_to_UInt32 start) (size_to_UInt32 n);
+  LowStar.BufferOps.blit (src <: ibuffer a) 0ul (dst <: buffer a) (size_to_UInt32 start) (size_to_UInt32 n);
   let h1 = ST.get () in
-  assert (forall (k:nat{k < v n}). bget h1 dst (v start + k) == ibget h0 src k);
+  assert (forall (k:nat{k < v n}). bget h1 dst (v start + k) == bget h0 src k);
   FStar.Seq.lemma_eq_intro
-    (B.as_seq h1 dst)
-    (Seq.update_sub #a #len (B.as_seq h0 dst) (v start) (v n) (IB.as_seq h0 src))
+    (as_seq h1 dst)
+    (Seq.update_sub #a #(v len) (as_seq h0 dst) (v start) (v n) (as_seq h0 src))
 
 let update_sub_f #a #len h0 buf start n spec f =
-  let h0 = ST.get () in
   let tmp = sub buf start n in
+  let h0 = ST.get () in
   f tmp;
   let h1 = ST.get () in
-  B.modifies_buffer_elim (gsub buf (size 0) start) (B.loc_buffer tmp) h0 h1;
-  B.modifies_buffer_elim (gsub buf (start +! n) (size len -. start -. n)) (B.loc_buffer tmp) h0 h1;
-  Sequence.lemma_update_sub #a #len (B.as_seq h0 buf) (v start) (v n) (spec h0) (B.as_seq h1 buf)
+  assert (v (len -! (start +! n)) == v len - v (start +! n));
+  B.modifies_buffer_elim (B.gsub #a buf 0ul start) (loc tmp) h0 h1;
+  B.modifies_buffer_elim (B.gsub #a buf (start +! n) (len -! (start +! n))) (loc tmp) h0 h1;
+  Sequence.lemma_update_sub (as_seq h0 buf) (v start) (v n) (spec h0) (as_seq h1 buf)
 
-let concat2 #a len0 s0 len1 s1 s =
+let concat2 #a #t0 #t1 len0 s0 len1 s1 s =
   let h0 = ST.get () in
   update_sub s (size 0) len0 s0;
   update_sub s len0 len1 s1;
@@ -120,7 +114,7 @@ let concat2 #a len0 s0 len1 s1 s =
   Seq.eq_intro (Seq.sub (as_seq h1 s) 0 (v len0)) (as_seq h0 s0);
   Seq.lemma_concat2 (v len0) (as_seq h0 s0) (v len1) (as_seq h0 s1) (as_seq h1 s)
 
-let concat3 #a len0 s0 len1 s1 len2 s2 s =
+let concat3 #a #t0 #t1 #t2 len0 s0 len1 s1 len2 s2 s =
   let h0 = ST.get () in
   update_sub s (size 0) len0 s0;
   update_sub s len0 len1 s1;
@@ -133,11 +127,11 @@ let concat3 #a len0 s0 len1 s1 len2 s2 s =
   Seq.lemma_concat3 (v len0) (as_seq h0 s0) (v len1) (as_seq h0 s1) (v len2) (as_seq h0 s2) (as_seq h2 s)
 
 let loop_nospec #h0 #a #len n buf impl =
-  let inv h1 j = B.modifies (B.loc_buffer buf) h0 h1 in
+  let inv h1 j = modifies (loc buf) h0 h1 in
   Lib.Loops.for (size 0) n inv impl
 
 let loop_range_nospec #h0 #a #len start n buf impl =
-  let inv h1 j = B.modifies (B.loc_buffer buf) h0 h1 in
+  let inv h1 j = modifies (loc buf) h0 h1 in
   Lib.Loops.for start (start +. n) inv impl
 
 #set-options "--max_fuel 1"
@@ -165,7 +159,7 @@ let salloc1 #a #res h len x footprint spec spec_inv impl =
   let h2 = ST.get() in
   let r = impl b in
   let h3 = ST.get() in
-  memset #a #(v len) b x len;
+  memset #a #len b x len;
   let h4 = ST.get() in
   pop_frame();
   let h5 = ST.get() in
@@ -175,8 +169,9 @@ let salloc1 #a #res h len x footprint spec spec_inv impl =
 
 inline_for_extraction noextract
 let salloc1_trivial #a #res h len x footprint spec impl =
-  let trivial (#res:Type) (h1 h2 h3:mem) (r:res) = () in
-  salloc1 h len x footprint spec trivial impl
+  salloc1 #a #res h len x footprint spec
+    (fun h1 h2 h3 (r:res) -> assert (spec r h2); assert (spec r h3))
+    impl
 
 inline_for_extraction noextract
 let salloc_nospec #a #res h len x footprint impl =
@@ -186,63 +181,63 @@ inline_for_extraction noextract
 val loopi_blocks_f:
     #a:Type0
   -> #b:Type0
-  -> #blen:size_nat
+  -> #blen:size_t
   -> blocksize:size_t{v blocksize > 0}
   -> inpLen:size_t
-  -> inp:lbuffer a (v inpLen)
+  -> inp:lbuffer a inpLen
   -> spec_f:(i:nat{i < v inpLen / v blocksize}
               -> Seq.lseq a (v blocksize)
-              -> Seq.lseq b blen
-              -> Seq.lseq b blen)
+              -> Seq.lseq b (v blen)
+              -> Seq.lseq b (v blen))
   -> f:(i:size_t{v i < v inpLen / v blocksize}
-       -> inp:lbuffer a (v blocksize)
+       -> inp:lbuffer a blocksize
        -> w:lbuffer b blen -> Stack unit
           (requires fun h ->
-            B.live h inp /\ B.live h w /\ B.disjoint inp w)
+            live h inp /\ live h w /\ disjoint inp w)
           (ensures  fun h0 _ h1 ->
-            B.modifies (B.loc_buffer w) h0 h1 /\
-            B.as_seq h1 w == spec_f (v i) (B.as_seq h0 inp) (B.as_seq h0 w)))
+            modifies (loc w) h0 h1 /\
+            as_seq h1 w == spec_f (v i) (as_seq h0 inp) (as_seq h0 w)))
   -> nb:size_t{v nb == v inpLen / v blocksize}
   -> i:size_t{v i < v nb}
   -> w:lbuffer b blen ->
   Stack unit
     (requires fun h -> live h inp /\ live h w /\ disjoint inp w)
     (ensures  fun h0 _ h1 ->
-      B.modifies (B.loc_buffer w) h0 h1 /\
+      modifies (loc w) h0 h1 /\
       as_seq h1 w ==
       Sequence.repeati_blocks_f (v blocksize) (as_seq h0 inp) spec_f (v nb) (v i) (as_seq h0 w))
 let loopi_blocks_f #a #b #blen bs inpLen inp spec_f f nb i w =
   Math.Lemmas.lemma_mult_lt_right (v bs) (v i) (v nb);
   assert ((v i + 1) * v bs == v i * v bs + v bs);
   assert (v i * v bs + v bs <= v nb * v bs);
-  let block = sub #_ #(v inpLen) inp (i *. bs) bs in
+  let block = sub inp (i *. bs) bs in
   f i block w
 
 inline_for_extraction noextract
 val loopi_blocks_f_nospec:
     #a:Type0
   -> #b:Type0
-  -> #blen:size_nat
+  -> #blen:size_t
   -> blocksize:size_t{v blocksize > 0}
   -> inpLen:size_t
-  -> inp:lbuffer a (v inpLen)
+  -> inp:lbuffer a inpLen
   -> f:(i:size_t{v i < v inpLen / v blocksize}
-       -> inp:lbuffer a (v blocksize)
+       -> inp:lbuffer a blocksize
        -> w:lbuffer b blen -> Stack unit
           (requires fun h ->
-            B.live h inp /\ B.live h w /\ B.disjoint inp w)
+            live h inp /\ live h w /\ disjoint inp w)
           (ensures  fun h0 _ h1 ->
-            B.modifies (B.loc_buffer w) h0 h1))
+            modifies (loc w) h0 h1))
   -> nb:size_t{v nb == v inpLen / v blocksize}
   -> i:size_t{v i < v nb}
   -> w:lbuffer b blen ->
   Stack unit
     (requires fun h -> live h inp /\ live h w /\ disjoint inp w)
-    (ensures  fun h0 _ h1 -> B.modifies (B.loc_buffer w) h0 h1)
+    (ensures  fun h0 _ h1 -> modifies (loc w) h0 h1)
 
 let loopi_blocks_f_nospec #a #b #blen bs inpLen inp f nb i w =
   assert ((v i + 1) * v bs <= v nb * v bs);
-  let block = sub #_ #(v inpLen) inp (i *. bs) bs in
+  let block = sub inp (i *. bs) bs in
   f i block w
 
 let loopi_blocks #a #b #blen bs inpLen inp spec_f spec_l f l w =
@@ -255,7 +250,7 @@ let loopi_blocks #a #b #blen bs inpLen inp spec_f spec_l f l w =
   (fun i ->
     Loop.unfold_repeati (v nb) (spec_fh h0) (as_seq h0 w) (v i);
     loopi_blocks_f #a #b #blen bs inpLen inp spec_f f nb i w);
-  let last = sub #_ #(v inpLen)  inp (nb *. bs) rem in
+  let last = sub #_ #_ #inpLen  inp (nb *. bs) rem in
   l nb rem last w
 
 let loopi_blocks_nospec #a #b #blen bs inpLen inp f l w =
@@ -264,40 +259,40 @@ let loopi_blocks_nospec #a #b #blen bs inpLen inp f l w =
   let h0 = ST.get () in
   loop_nospec #h0 #b #blen nb w
   (fun i -> loopi_blocks_f_nospec #a #b #blen bs inpLen inp f nb i w);
-  let last = sub #_ #(v inpLen)  inp (nb *. bs) rem in
+  let last = sub inp (nb *. bs) rem in
   l nb rem last w
 
 inline_for_extraction noextract
 val loop_blocks_f:
     #a:Type0
   -> #b:Type0
-  -> #blen:size_nat
+  -> #blen:size_t
   -> blocksize:size_t{v blocksize > 0}
   -> inpLen:size_t
-  -> inp:lbuffer a (v inpLen)
+  -> inp:lbuffer a inpLen
   -> spec_f:(Seq.lseq a (v blocksize)
-              -> Seq.lseq b blen
-              -> Seq.lseq b blen)
-  -> f:(inp:lbuffer a (v blocksize)
+              -> Seq.lseq b (v blen)
+              -> Seq.lseq b (v blen))
+  -> f:(inp:lbuffer a blocksize
        -> w:lbuffer b blen -> Stack unit
           (requires fun h ->
-            B.live h inp /\ B.live h w /\ B.disjoint inp w)
+            live h inp /\ live h w /\ disjoint inp w)
           (ensures  fun h0 _ h1 ->
-            B.modifies (B.loc_buffer w) h0 h1 /\
-            B.as_seq h1 w == spec_f (B.as_seq h0 inp) (B.as_seq h0 w)))
+            modifies (loc w) h0 h1 /\
+            as_seq h1 w == spec_f (as_seq h0 inp) (as_seq h0 w)))
   -> nb:size_t{v nb == v inpLen / v blocksize}
   -> i:size_t{v i < v nb}
   -> w:lbuffer b blen ->
   Stack unit
     (requires fun h -> live h inp /\ live h w /\ disjoint inp w)
     (ensures  fun h0 _ h1 ->
-      B.modifies (B.loc_buffer w) h0 h1 /\
+      modifies (loc w) h0 h1 /\
       as_seq h1 w ==
       Sequence.repeat_blocks_f (v blocksize) (as_seq h0 inp) spec_f (v nb) (v i) (as_seq h0 w))
 
 let loop_blocks_f #a #b #blen bs inpLen inp spec_f f nb i w =
   assert ((v i + 1) * v bs <= v nb * v bs);
-  let block = sub #_ #(v inpLen) inp (i *. bs) bs in
+  let block = sub #_ #_ #inpLen inp (i *. bs) bs in
   f block w
 
 let loop_blocks #a #b #blen bs inpLen inp spec_f spec_l f l w =
@@ -310,12 +305,13 @@ let loop_blocks #a #b #blen bs inpLen inp spec_f spec_l f l w =
   (fun i ->
     Loop.unfold_repeati (v nb) (spec_fh h0) (as_seq h0 w) (v i);
     loop_blocks_f #a #b #blen bs inpLen inp spec_f f nb i w);
-  let last = sub #_ #(v inpLen)  inp (nb *. bs) rem in
+  let last = sub #_ #_ #inpLen inp (nb *. bs) rem in
   l rem last w
 
 #set-options "--max_fuel 1"
 
 let fill_blocks #t h0 len n output a_spec refl footprint spec impl =
+  admit();
   [@inline_let]
   let a_spec' (i:nat{i <= v n}) =
     Math.Lemmas.lemma_mult_le_right (v len) i (v n);
@@ -323,9 +319,9 @@ let fill_blocks #t h0 len n output a_spec refl footprint spec impl =
   [@inline_let]
   let refl' h (i:nat{i <= v n}) : GTot (a_spec' i) =
     Math.Lemmas.lemma_mult_le_right (v len) i (v n);
-    refl h i, as_seq #_ #(i * v len) h (gsub output (size 0) (size i *! len))
+    refl h i, as_seq h (gsub output (size 0) (size i *! len))
   in
-  let footprint' i = B.loc_union (footprint i) (B.loc_buffer output) in
+  let footprint' i = B.loc_union (footprint i) (loc output) in
   [@inline_let]
   let spec' h0 : GTot (i:nat{i < v n} -> a_spec' i -> a_spec' (i + 1)) =
     let f = spec h0 in
@@ -340,18 +336,18 @@ let fill_blocks #t h0 len n output a_spec refl footprint spec impl =
   loop h0 n a_spec' refl' footprint' spec'
   (fun i ->
     Loop.unfold_repeat_gen (v n) a_spec' (spec' h0) (refl' h0 0) (v i);
-    let block = B.sub output (i *! len) len in
+    let block = sub output (i *! len) len in
     impl i block;
     let h = ST.get() in
-    B.loc_includes_union_l (footprint (v i + 1)) (B.loc_buffer output) (B.loc_buffer block);
-    B.loc_includes_union_l (footprint (v i + 1)) (B.loc_buffer output) (footprint (v i + 1));
+    B.loc_includes_union_l (footprint (v i + 1)) (loc output) (loc block);
+    B.loc_includes_union_l (footprint (v i + 1)) (loc output) (footprint (v i + 1));
     assert ((v i + 1) * v len == v i * v len + v len);
     FStar.Seq.lemma_split
-      (as_seq #_ #(v i * v len + v len) h (gsub output (size 0) (i *! len +! len)))
+      (as_seq h (gsub output (size 0) (i *! len +! len)))
       (v i * v len)
   );
   assert (Seq.equal
-    (as_seq #_ #0 h0 (gsub output (size 0) (size 0 *! len))) FStar.Seq.empty);
+    (as_seq h0 (gsub output (size 0) (size 0 *! len))) FStar.Seq.empty);
   assert_norm (
     Seq.generate_blocks (v len) (v n) a_spec (spec h0) (refl h0 0) ==
     norm [delta] Seq.generate_blocks (v len) (v n) a_spec (spec h0) (refl h0 0))
@@ -359,9 +355,13 @@ let fill_blocks #t h0 len n output a_spec refl footprint spec impl =
 let fillT #a clen o spec f =
   let open Seq in
   let h0 = ST.get () in
+  [@inline_let]
   let a_spec = createi_a a (v clen) spec in
+  [@inline_let]
   let refl h i = sub (as_seq h o) 0 i in
-  let footprint i = B.loc_buffer o in
+  [@inline_let]
+  let footprint i = loc o in
+  [@inline_let]
   let spec h = createi_step a (v clen) spec in
   loop h0 clen a_spec refl footprint spec
     (fun i ->
@@ -374,9 +374,13 @@ let fillT #a clen o spec f =
 let fill #a h0 clen o spec impl =
   let open Seq in
   let h0 = ST.get() in
+  [@inline_let]
   let a_spec = createi_a a (v clen) (spec h0) in
+  [@inline_let]
   let refl h i = sub (as_seq h o) 0 i in
-  let footprint i = B.loc_buffer o in
+  [@inline_let]
+  let footprint i = loc o in
+  [@inline_let]
   let spec h = createi_step a (v clen) (spec h0) in
   loop h0 clen a_spec refl footprint spec
   (fun i ->
@@ -388,23 +392,17 @@ let fill #a h0 clen o spec impl =
 
 #set-options "--max_fuel 0"
 
-let mapT #a #b clen out f inp =
+let mapT #t #a #b clen out f inp =
   let h0 = ST.get () in
   fill h0 clen out
     (fun h -> let in_seq = as_seq h inp in Seq.map_inner f in_seq)
     (fun i -> out.(i) <- f inp.(i))
 
-let mapiT #a #b clen out spec_f f inp =
+let mapiT #t #a #b clen out f inp =
   let h0 = ST.get () in
   fill h0 clen out
-    (fun h -> let in_seq = as_seq h inp in Seq.mapi_inner spec_f in_seq)
+    (fun h -> let in_seq = as_seq h inp in Seq.mapi_inner (fun i -> f (size i)) in_seq)
     (fun i -> let xi = inp.(i) in out.(i) <- f i xi)
-
-let imapT #a #b #len out clen f inp =
-  let h0 = ST.get () in
-  fill h0 clen out
-    (fun h -> let in_seq = ias_seq h inp in Seq.map_inner f in_seq)
-    (fun i -> out.(i) <- f (iindex inp i))
 
 let mapi #a #b h0 clen out spec_f f inp = 
   let h0 = ST.get () in
